src/tactics/FStar.Tactics.V1.Basic.fst
@@ -56,6 +56,7 @@ module UF     = FStar.Syntax.Unionfind
 module U      = FStar.Syntax.Util
 module Z      = FStar.BigInt
 module Core   = FStar.TypeChecker.Core
+module PO     = FStar.TypeChecker.Primops
 
 let core_check env sol t must_tot
   : either (option typ) Core.error
@@ -144,7 +145,7 @@ let debugging () : tac bool =
 
 let do_dump_ps (msg:string) (ps:proofstate) : unit =
   let psc = ps.psc in
-  let subst = Cfg.psc_subst psc in
+  let subst = PO.psc_subst psc in
   do_dump_proofstate ps msg
 
 let dump (msg:string) : tac unit =
