src/tactics/FStar.Tactics.Types.fsti
@@ -19,13 +19,14 @@ open FStar.Compiler.Effect
 open FStar.Syntax.Syntax
 open FStar.TypeChecker.Env
 open FStar.Tactics.Common
-module Cfg = FStar.TypeChecker.Cfg
-module N = FStar.TypeChecker.Normalize
-module Range = FStar.Compiler.Range
-module BU = FStar.Compiler.Util
-module O = FStar.Options
 
-module Core = FStar.TypeChecker.Core
+module BU      = FStar.Compiler.Util
+module Cfg     = FStar.TypeChecker.Cfg
+module Core    = FStar.TypeChecker.Core
+module N       = FStar.TypeChecker.Normalize
+module O       = FStar.Options
+module PO      = FStar.TypeChecker.Primops
+module Range   = FStar.Compiler.Range
 
 (*
    f: x:int -> P
@@ -67,7 +68,7 @@ type proofstate = {
 
     depth        : int;          //depth for tracing and debugging
     __dump       : proofstate -> string -> unit; // callback to dump_proofstate, to avoid an annoying circularity
-    psc          : Cfg.psc;        //primitive step context where we started execution
+    psc          : PO.psc;       //primitive step context where we started execution
     entry_range  : Range.range;  //position of entry, set by the use
     guard_policy : guard_policy; //guard policy: what to do with guards arising during tactic exec
     freshness    : int;          //a simple freshness counter for the fresh tactic
@@ -82,11 +83,11 @@ type proofstate = {
 
 val decr_depth : proofstate -> proofstate
 val incr_depth : proofstate -> proofstate
-val tracepoint_with_psc : Cfg.psc -> proofstate -> bool
+val tracepoint_with_psc : PO.psc -> proofstate -> bool
 val tracepoint : proofstate -> bool
 val set_proofstate_range : proofstate -> Range.range -> proofstate
 
-val set_ps_psc : Cfg.psc -> proofstate -> proofstate
+val set_ps_psc : PO.psc -> proofstate -> proofstate
 val goal_env: goal -> env
 val goal_range: goal -> Range.range
 val goal_witness: goal -> term
