src/tactics/FStar.Tactics.V2.InterpFuns.fst
@@ -38,6 +38,7 @@ module Cfg   = FStar.TypeChecker.Cfg
 module E     = FStar.Tactics.Embedding
 module NBETerm = FStar.TypeChecker.NBETerm
 module NBET    = FStar.TypeChecker.NBETerm
+module PO    = FStar.TypeChecker.Primops
 
 let unembed e t n = FStar.Syntax.Embeddings.unembed e t n
 let embed e rng t n = FStar.Syntax.Embeddings.embed e t rng None n
@@ -63,38 +64,38 @@ let timing_nbe (l:Ident.lid) f =
         (* BU.print1 "%s }\n" (Ident.string_of_lid l); *)
         r
 
-let mk nm arity nunivs interp nbe_interp =
+let mk nm arity nunivs interp nbe_interp : PO.primitive_step =
   let nm = PC.fstar_tactics_lid' ["V2"; "Builtins"; nm] in
-  { Cfg.name                         = nm
-  ; Cfg.arity                        = arity
-  ; Cfg.univ_arity                   = nunivs
-  ; Cfg.auto_reflect                 = Some (arity - 1)
-  ; Cfg.strong_reduction_ok          = true
-  ; Cfg.requires_binder_substitution = true
-  ; Cfg.renorm_after                 = false
-  ; Cfg.interpretation               = (fun psc cbs _us args -> timing_int nm interp psc cbs args)
-  ; Cfg.interpretation_nbe           = (fun cbs _us args -> timing_nbe nm nbe_interp cbs args)
+  { name                         = nm
+  ; arity                        = arity
+  ; univ_arity                   = nunivs
+  ; auto_reflect                 = Some (arity - 1)
+  ; strong_reduction_ok          = true
+  ; requires_binder_substitution = true
+  ; renorm_after                 = false
+  ; interpretation               = (fun psc cbs _us args -> timing_int nm interp psc cbs args)
+  ; interpretation_nbe           = (fun cbs _us args -> timing_nbe nm nbe_interp cbs args)
   }
 
-let mkt nm arity nunivs interp nbe_interp =
+let mkt nm arity nunivs interp nbe_interp : PO.primitive_step =
   let nm = PC.fstar_tactics_lid' ["V2"; "Builtins"; nm] in
-  { Cfg.name                         = nm
-  ; Cfg.arity                        = arity
-  ; Cfg.univ_arity                   = nunivs
-  ; Cfg.auto_reflect                 = None
-  ; Cfg.strong_reduction_ok          = true
-  ; Cfg.requires_binder_substitution = true
-  ; Cfg.renorm_after                 = false
-  ; Cfg.interpretation               = (fun psc cbs _us args -> timing_int nm interp psc cbs args)
-  ; Cfg.interpretation_nbe           = (fun cbs _us args -> timing_nbe nm nbe_interp cbs args)
+  { name                         = nm
+  ; arity                        = arity
+  ; univ_arity                   = nunivs
+  ; auto_reflect                 = None
+  ; strong_reduction_ok          = true
+  ; requires_binder_substitution = true
+  ; renorm_after                 = false
+  ; interpretation               = (fun psc cbs _us args -> timing_int nm interp psc cbs args)
+  ; interpretation_nbe           = (fun cbs _us args -> timing_nbe nm nbe_interp cbs args)
   }
 
 (* This _psc variant is a special case *)
 let mk_total_interpretation_1_psc
-    (f:Cfg.psc -> 't1 -> 'r)
+    (f:PO.psc -> 't1 -> 'r)
     (e1: embedding 't1)
     (er:embedding 'r)
-    (psc:Cfg.psc)
+    (psc:PO.psc)
     (ncb:norm_cb)
     (args:args)
   : option term
@@ -103,13 +104,13 @@ let mk_total_interpretation_1_psc
   | [(a1, _)] ->
     BU.bind_opt (unembed e1 a1 ncb) (fun a1 ->
     let r = f psc a1 in
-    Some (embed er (Cfg.psc_range psc) r ncb))
+    Some (embed er (PO.psc_range psc) r ncb))
   | _ ->
     None
 
 let mk_total_nbe_interpretation_1_psc
     cb
-    (f:Cfg.psc -> 't1 -> 'r)
+    (f:PO.psc -> 't1 -> 'r)
     (e1: NBET.embedding 't1)
     (er:NBET.embedding 'r)
     (args:NBET.args)
@@ -118,19 +119,19 @@ let mk_total_nbe_interpretation_1_psc
   match args with
   | [(a1, _)] ->
     BU.bind_opt (NBET.unembed e1 cb a1) (fun a1 ->
-    let r = f Cfg.null_psc a1 in // TODO: no psc here?
+    let r = f PO.null_psc a1 in // TODO: no psc here?
     Some (NBET.embed er cb r))
   | _ ->
     None
 
 let mk_total_step_1_psc (nunivs:int) (name : string)
-           (f : Cfg.psc -> 'a -> 'r)
+           (f : PO.psc -> 'a -> 'r)
            (ea : embedding 'a)
            (er : embedding 'r)
-           (nf : Cfg.psc -> 'na -> 'nr)
+           (nf : PO.psc -> 'na -> 'nr)
            (nea : NBETerm.embedding 'na)
            (ner : NBETerm.embedding 'nr)
-           : Cfg.primitive_step =
+           : PO.primitive_step =
     mkt name 1 nunivs (mk_total_interpretation_1_psc     f  ea  er)
                       (fun cb args -> mk_total_nbe_interpretation_1_psc cb nf nea ner (drop nunivs args))
 
@@ -145,7 +146,7 @@ let mk_tactic_interpretation_1
     (t : 't1 -> tac 'r)
     (e1:embedding 't1)
     (er:embedding 'r)
-    (psc:Cfg.psc)
+    (psc:PO.psc)
     (ncb:norm_cb)
     (args:args)
   : option term
@@ -156,7 +157,7 @@ let mk_tactic_interpretation_1
     BU.bind_opt (unembed E.e_proofstate a2 ncb) (fun ps ->
     let ps = set_ps_psc psc ps in
     let r = interp_ctx name (fun () -> run_safe (t a1) ps) in
-    Some (embed (E.e_result er) (Cfg.psc_range psc) r ncb)))
+    Some (embed (E.e_result er) (PO.psc_range psc) r ncb)))
   | _ ->
     None
 
@@ -166,7 +167,7 @@ let mk_tactic_interpretation_2
     (e1:embedding 't1)
     (e2:embedding 't2)
     (er:embedding 'r)
-    (psc:Cfg.psc)
+    (psc:PO.psc)
     (ncb:norm_cb)
     (args:args)
   : option term
@@ -178,7 +179,7 @@ let mk_tactic_interpretation_2
     BU.bind_opt (unembed E.e_proofstate a3 ncb) (fun ps ->
     let ps = set_ps_psc psc ps in
     let r = interp_ctx name (fun () -> run_safe (t a1 a2) ps) in
-    Some (embed (E.e_result er) (Cfg.psc_range psc) r ncb))))
+    Some (embed (E.e_result er) (PO.psc_range psc) r ncb))))
   | _ ->
     None
 
@@ -189,7 +190,7 @@ let mk_tactic_interpretation_3
     (e2:embedding 't2)
     (e3:embedding 't3)
     (er:embedding 'r)
-    (psc:Cfg.psc)
+    (psc:PO.psc)
     (ncb:norm_cb)
     (args:args)
   : option term
@@ -202,7 +203,7 @@ let mk_tactic_interpretation_3
     BU.bind_opt (unembed E.e_proofstate a4 ncb) (fun ps ->
     let ps = set_ps_psc psc ps in
     let r = interp_ctx name (fun () -> run_safe (t a1 a2 a3) ps) in
-    Some (embed (E.e_result er) (Cfg.psc_range psc) r ncb)))))
+    Some (embed (E.e_result er) (PO.psc_range psc) r ncb)))))
   | _ ->
     None
 
@@ -214,7 +215,7 @@ let mk_tactic_interpretation_4
     (e3:embedding 't3)
     (e4:embedding 't4)
     (er:embedding 'r)
-    (psc:Cfg.psc)
+    (psc:PO.psc)
     (ncb:norm_cb)
     (args:args)
   : option term
@@ -228,7 +229,7 @@ let mk_tactic_interpretation_4
     BU.bind_opt (unembed E.e_proofstate a5 ncb) (fun ps ->
     let ps = set_ps_psc psc ps in
     let r = interp_ctx name (fun () -> run_safe (t a1 a2 a3 a4) ps) in
-    Some (embed (E.e_result er) (Cfg.psc_range psc) r ncb))))))
+    Some (embed (E.e_result er) (PO.psc_range psc) r ncb))))))
   | _ ->
     None
 
@@ -241,7 +242,7 @@ let mk_tactic_interpretation_5
     (e4:embedding 't4)
     (e5:embedding 't5)
     (er:embedding 'r)
-    (psc:Cfg.psc)
+    (psc:PO.psc)
     (ncb:norm_cb)
     (args:args)
   : option term
@@ -256,7 +257,7 @@ let mk_tactic_interpretation_5
     BU.bind_opt (unembed E.e_proofstate a6 ncb) (fun ps ->
     let ps = set_ps_psc psc ps in
     let r = interp_ctx name (fun () -> run_safe (t a1 a2 a3 a4 a5) ps) in
-    Some (embed (E.e_result er) (Cfg.psc_range psc) r ncb)))))))
+    Some (embed (E.e_result er) (PO.psc_range psc) r ncb)))))))
   | _ ->
     None
 
@@ -270,7 +271,7 @@ let mk_tactic_interpretation_6
     (e5:embedding 't5)
     (e6:embedding 't6)
     (er:embedding 'r)
-    (psc:Cfg.psc)
+    (psc:PO.psc)
     (ncb:norm_cb)
     (args:args)
   : option term
@@ -286,7 +287,7 @@ let mk_tactic_interpretation_6
     BU.bind_opt (unembed E.e_proofstate a7 ncb) (fun ps ->
     let ps = set_ps_psc psc ps in
     let r = interp_ctx name (fun () -> run_safe (t a1 a2 a3 a4 a5 a6) ps) in
-    Some (embed (E.e_result er) (Cfg.psc_range psc) r ncb))))))))
+    Some (embed (E.e_result er) (PO.psc_range psc) r ncb))))))))
   | _ ->
     None
 
@@ -301,7 +302,7 @@ let mk_tactic_interpretation_7
     (e6:embedding 't6)
     (e7:embedding 't7)
     (er:embedding 'r)
-    (psc:Cfg.psc)
+    (psc:PO.psc)
     (ncb:norm_cb)
     (args:args)
   : option term
@@ -318,7 +319,7 @@ let mk_tactic_interpretation_7
     BU.bind_opt (unembed E.e_proofstate a8 ncb) (fun ps ->
     let ps = set_ps_psc psc ps in
     let r = interp_ctx name (fun () -> run_safe (t a1 a2 a3 a4 a5 a6 a7) ps) in
-    Some (embed (E.e_result er) (Cfg.psc_range psc) r ncb)))))))))
+    Some (embed (E.e_result er) (PO.psc_range psc) r ncb)))))))))
   | _ ->
     None
 
@@ -334,7 +335,7 @@ let mk_tactic_interpretation_8
     (e7:embedding 't7)
     (e8:embedding 't8)
     (er:embedding 'r)
-    (psc:Cfg.psc)
+    (psc:PO.psc)
     (ncb:norm_cb)
     (args:args)
   : option term
@@ -352,7 +353,7 @@ let mk_tactic_interpretation_8
     BU.bind_opt (unembed E.e_proofstate a9 ncb) (fun ps ->
     let ps = set_ps_psc psc ps in
     let r = interp_ctx name (fun () -> run_safe (t a1 a2 a3 a4 a5 a6 a7 a8) ps) in
-    Some (embed (E.e_result er) (Cfg.psc_range psc) r ncb))))))))))
+    Some (embed (E.e_result er) (PO.psc_range psc) r ncb))))))))))
   | _ ->
     None
 
@@ -369,7 +370,7 @@ let mk_tactic_interpretation_9
     (e8:embedding 't8)
     (e9:embedding 't9)
     (er:embedding 'r)
-    (psc:Cfg.psc)
+    (psc:PO.psc)
     (ncb:norm_cb)
     (args:args)
   : option term
@@ -388,7 +389,7 @@ let mk_tactic_interpretation_9
     BU.bind_opt (unembed E.e_proofstate a10 ncb) (fun ps ->
     let ps = set_ps_psc psc ps in
     let r = interp_ctx name (fun () -> run_safe (t a1 a2 a3 a4 a5 a6 a7 a8 a9) ps) in
-    Some (embed (E.e_result er) (Cfg.psc_range psc) r ncb)))))))))))
+    Some (embed (E.e_result er) (PO.psc_range psc) r ncb)))))))))))
   | _ ->
     None
 
@@ -406,7 +407,7 @@ let mk_tactic_interpretation_10
     (e9:embedding 't9)
     (e10:embedding 't10)
     (er:embedding 'r)
-    (psc:Cfg.psc)
+    (psc:PO.psc)
     (ncb:norm_cb)
     (args:args)
   : option term
@@ -426,7 +427,7 @@ let mk_tactic_interpretation_10
     BU.bind_opt (unembed E.e_proofstate a11 ncb) (fun ps ->
     let ps = set_ps_psc psc ps in
     let r = interp_ctx name (fun () -> run_safe (t a1 a2 a3 a4 a5 a6 a7 a8 a9 a10) ps) in
-    Some (embed (E.e_result er) (Cfg.psc_range psc) r ncb))))))))))))
+    Some (embed (E.e_result er) (PO.psc_range psc) r ncb))))))))))))
   | _ ->
     None
 
@@ -445,7 +446,7 @@ let mk_tactic_interpretation_11
     (e10:embedding 't10)
     (e11:embedding 't11)
     (er:embedding 'r)
-    (psc:Cfg.psc)
+    (psc:PO.psc)
     (ncb:norm_cb)
     (args:args)
   : option term
@@ -466,7 +467,7 @@ let mk_tactic_interpretation_11
     BU.bind_opt (unembed E.e_proofstate a12 ncb) (fun ps ->
     let ps = set_ps_psc psc ps in
     let r = interp_ctx name (fun () -> run_safe (t a1 a2 a3 a4 a5 a6 a7 a8 a9 a10 a11) ps) in
-    Some (embed (E.e_result er) (Cfg.psc_range psc) r ncb)))))))))))))
+    Some (embed (E.e_result er) (PO.psc_range psc) r ncb)))))))))))))
   | _ ->
     None
 
@@ -486,7 +487,7 @@ let mk_tactic_interpretation_12
     (e11:embedding 't11)
     (e12:embedding 't12)
     (er:embedding 'r)
-    (psc:Cfg.psc)
+    (psc:PO.psc)
     (ncb:norm_cb)
     (args:args)
   : option term
@@ -508,7 +509,7 @@ let mk_tactic_interpretation_12
     BU.bind_opt (unembed E.e_proofstate a13 ncb) (fun ps ->
     let ps = set_ps_psc psc ps in
     let r = interp_ctx name (fun () -> run_safe (t a1 a2 a3 a4 a5 a6 a7 a8 a9 a10 a11 a12) ps) in
-    Some (embed (E.e_result er) (Cfg.psc_range psc) r ncb))))))))))))))
+    Some (embed (E.e_result er) (PO.psc_range psc) r ncb))))))))))))))
   | _ ->
     None
 
@@ -529,7 +530,7 @@ let mk_tactic_interpretation_13
     (e12:embedding 't12)
     (e13:embedding 't13)
     (er:embedding 'r)
-    (psc:Cfg.psc)
+    (psc:PO.psc)
     (ncb:norm_cb)
     (args:args)
   : option term
@@ -552,7 +553,7 @@ let mk_tactic_interpretation_13
     BU.bind_opt (unembed E.e_proofstate a14 ncb) (fun ps ->
     let ps = set_ps_psc psc ps in
     let r = interp_ctx name (fun () -> run_safe (t a1 a2 a3 a4 a5 a6 a7 a8 a9 a10 a11 a12 a13) ps) in
-    Some (embed (E.e_result er) (Cfg.psc_range psc) r ncb)))))))))))))))
+    Some (embed (E.e_result er) (PO.psc_range psc) r ncb)))))))))))))))
   | _ ->
     None
 
@@ -574,7 +575,7 @@ let mk_tactic_interpretation_14
     (e13:embedding 't13)
     (e14:embedding 't14)
     (er:embedding 'r)
-    (psc:Cfg.psc)
+    (psc:PO.psc)
     (ncb:norm_cb)
     (args:args)
   : option term
@@ -598,7 +599,7 @@ let mk_tactic_interpretation_14
     BU.bind_opt (unembed E.e_proofstate a15 ncb) (fun ps ->
     let ps = set_ps_psc psc ps in
     let r = interp_ctx name (fun () -> run_safe (t a1 a2 a3 a4 a5 a6 a7 a8 a9 a10 a11 a12 a13 a14) ps) in
-    Some (embed (E.e_result er) (Cfg.psc_range psc) r ncb))))))))))))))))
+    Some (embed (E.e_result er) (PO.psc_range psc) r ncb))))))))))))))))
   | _ ->
     None
 
@@ -621,7 +622,7 @@ let mk_tactic_interpretation_15
     (e14:embedding 't14)
     (e15:embedding 't15)
     (er:embedding 'r)
-    (psc:Cfg.psc)
+    (psc:PO.psc)
     (ncb:norm_cb)
     (args:args)
   : option term
@@ -646,7 +647,7 @@ let mk_tactic_interpretation_15
     BU.bind_opt (unembed E.e_proofstate a16 ncb) (fun ps ->
     let ps = set_ps_psc psc ps in
     let r = interp_ctx name (fun () -> run_safe (t a1 a2 a3 a4 a5 a6 a7 a8 a9 a10 a11 a12 a13 a14 a15) ps) in
-    Some (embed (E.e_result er) (Cfg.psc_range psc) r ncb)))))))))))))))))
+    Some (embed (E.e_result er) (PO.psc_range psc) r ncb)))))))))))))))))
   | _ ->
     None
 
@@ -670,7 +671,7 @@ let mk_tactic_interpretation_16
     (e15:embedding 't15)
     (e16:embedding 't16)
     (er:embedding 'r)
-    (psc:Cfg.psc)
+    (psc:PO.psc)
     (ncb:norm_cb)
     (args:args)
   : option term
@@ -696,7 +697,7 @@ let mk_tactic_interpretation_16
     BU.bind_opt (unembed E.e_proofstate a17 ncb) (fun ps ->
     let ps = set_ps_psc psc ps in
     let r = interp_ctx name (fun () -> run_safe (t a1 a2 a3 a4 a5 a6 a7 a8 a9 a10 a11 a12 a13 a14 a15 a16) ps) in
-    Some (embed (E.e_result er) (Cfg.psc_range psc) r ncb))))))))))))))))))
+    Some (embed (E.e_result er) (PO.psc_range psc) r ncb))))))))))))))))))
   | _ ->
     None
 
@@ -721,7 +722,7 @@ let mk_tactic_interpretation_17
     (e16:embedding 't16)
     (e17:embedding 't17)
     (er:embedding 'r)
-    (psc:Cfg.psc)
+    (psc:PO.psc)
     (ncb:norm_cb)
     (args:args)
   : option term
@@ -748,7 +749,7 @@ let mk_tactic_interpretation_17
     BU.bind_opt (unembed E.e_proofstate a18 ncb) (fun ps ->
     let ps = set_ps_psc psc ps in
     let r = interp_ctx name (fun () -> run_safe (t a1 a2 a3 a4 a5 a6 a7 a8 a9 a10 a11 a12 a13 a14 a15 a16 a17) ps) in
-    Some (embed (E.e_result er) (Cfg.psc_range psc) r ncb)))))))))))))))))))
+    Some (embed (E.e_result er) (PO.psc_range psc) r ncb)))))))))))))))))))
   | _ ->
     None
 
@@ -774,7 +775,7 @@ let mk_tactic_interpretation_18
     (e17:embedding 't17)
     (e18:embedding 't18)
     (er:embedding 'r)
-    (psc:Cfg.psc)
+    (psc:PO.psc)
     (ncb:norm_cb)
     (args:args)
   : option term
@@ -802,7 +803,7 @@ let mk_tactic_interpretation_18
     BU.bind_opt (unembed E.e_proofstate a19 ncb) (fun ps ->
     let ps = set_ps_psc psc ps in
     let r = interp_ctx name (fun () -> run_safe (t a1 a2 a3 a4 a5 a6 a7 a8 a9 a10 a11 a12 a13 a14 a15 a16 a17 a18) ps) in
-    Some (embed (E.e_result er) (Cfg.psc_range psc) r ncb))))))))))))))))))))
+    Some (embed (E.e_result er) (PO.psc_range psc) r ncb))))))))))))))))))))
   | _ ->
     None
 
@@ -829,7 +830,7 @@ let mk_tactic_interpretation_19
     (e18:embedding 't18)
     (e19:embedding 't19)
     (er:embedding 'r)
-    (psc:Cfg.psc)
+    (psc:PO.psc)
     (ncb:norm_cb)
     (args:args)
   : option term
@@ -858,7 +859,7 @@ let mk_tactic_interpretation_19
     BU.bind_opt (unembed E.e_proofstate a20 ncb) (fun ps ->
     let ps = set_ps_psc psc ps in
     let r = interp_ctx name (fun () -> run_safe (t a1 a2 a3 a4 a5 a6 a7 a8 a9 a10 a11 a12 a13 a14 a15 a16 a17 a18 a19) ps) in
-    Some (embed (E.e_result er) (Cfg.psc_range psc) r ncb)))))))))))))))))))))
+    Some (embed (E.e_result er) (PO.psc_range psc) r ncb)))))))))))))))))))))
   | _ ->
     None
 
@@ -886,7 +887,7 @@ let mk_tactic_interpretation_20
     (e19:embedding 't19)
     (e20:embedding 't20)
     (er:embedding 'r)
-    (psc:Cfg.psc)
+    (psc:PO.psc)
     (ncb:norm_cb)
     (args:args)
   : option term
@@ -916,7 +917,7 @@ let mk_tactic_interpretation_20
     BU.bind_opt (unembed E.e_proofstate a21 ncb) (fun ps ->
     let ps = set_ps_psc psc ps in
     let r = interp_ctx name (fun () -> run_safe (t a1 a2 a3 a4 a5 a6 a7 a8 a9 a10 a11 a12 a13 a14 a15 a16 a17 a18 a19 a20) ps) in
-    Some (embed (E.e_result er) (Cfg.psc_range psc) r ncb))))))))))))))))))))))
+    Some (embed (E.e_result er) (PO.psc_range psc) r ncb))))))))))))))))))))))
   | _ ->
     None
 
@@ -1665,7 +1666,7 @@ let mk_total_interpretation_1
     (f : 't1 -> 'r)
     (e1:embedding 't1)
     (er:embedding 'r)
-    (psc:Cfg.psc)
+    (psc:PO.psc)
     (ncb:norm_cb)
     (args:args)
   : option term
@@ -1674,7 +1675,7 @@ let mk_total_interpretation_1
   | [(a1, _)] ->
     BU.bind_opt (unembed e1 a1 ncb) (fun a1 ->
     let r = interp_ctx name (fun () -> f a1) in
-    Some (embed er (Cfg.psc_range psc) r ncb))
+    Some (embed er (PO.psc_range psc) r ncb))
   | _ ->
     None
 
@@ -1684,7 +1685,7 @@ let mk_total_interpretation_2
     (e1:embedding 't1)
     (e2:embedding 't2)
     (er:embedding 'r)
-    (psc:Cfg.psc)
+    (psc:PO.psc)
     (ncb:norm_cb)
     (args:args)
   : option term
@@ -1694,7 +1695,7 @@ let mk_total_interpretation_2
     BU.bind_opt (unembed e1 a1 ncb) (fun a1 ->
     BU.bind_opt (unembed e2 a2 ncb) (fun a2 ->
     let r = interp_ctx name (fun () -> f a1 a2) in
-    Some (embed er (Cfg.psc_range psc) r ncb)))
+    Some (embed er (PO.psc_range psc) r ncb)))
   | _ ->
     None
 
@@ -1705,7 +1706,7 @@ let mk_total_interpretation_3
     (e2:embedding 't2)
     (e3:embedding 't3)
     (er:embedding 'r)
-    (psc:Cfg.psc)
+    (psc:PO.psc)
     (ncb:norm_cb)
     (args:args)
   : option term
@@ -1716,7 +1717,7 @@ let mk_total_interpretation_3
     BU.bind_opt (unembed e2 a2 ncb) (fun a2 ->
     BU.bind_opt (unembed e3 a3 ncb) (fun a3 ->
     let r = interp_ctx name (fun () -> f a1 a2 a3) in
-    Some (embed er (Cfg.psc_range psc) r ncb))))
+    Some (embed er (PO.psc_range psc) r ncb))))
   | _ ->
     None
 
@@ -1728,7 +1729,7 @@ let mk_total_interpretation_4
     (e3:embedding 't3)
     (e4:embedding 't4)
     (er:embedding 'r)
-    (psc:Cfg.psc)
+    (psc:PO.psc)
     (ncb:norm_cb)
     (args:args)
   : option term
@@ -1740,7 +1741,7 @@ let mk_total_interpretation_4
     BU.bind_opt (unembed e3 a3 ncb) (fun a3 ->
     BU.bind_opt (unembed e4 a4 ncb) (fun a4 ->
     let r = interp_ctx name (fun () -> f a1 a2 a3 a4) in
-    Some (embed er (Cfg.psc_range psc) r ncb)))))
+    Some (embed er (PO.psc_range psc) r ncb)))))
   | _ ->
     None
 
@@ -1753,7 +1754,7 @@ let mk_total_interpretation_5
     (e4:embedding 't4)
     (e5:embedding 't5)
     (er:embedding 'r)
-    (psc:Cfg.psc)
+    (psc:PO.psc)
     (ncb:norm_cb)
     (args:args)
   : option term
@@ -1766,7 +1767,7 @@ let mk_total_interpretation_5
     BU.bind_opt (unembed e4 a4 ncb) (fun a4 ->
     BU.bind_opt (unembed e5 a5 ncb) (fun a5 ->
     let r = interp_ctx name (fun () -> f a1 a2 a3 a4 a5) in
-    Some (embed er (Cfg.psc_range psc) r ncb))))))
+    Some (embed er (PO.psc_range psc) r ncb))))))
   | _ ->
     None
 
@@ -1780,7 +1781,7 @@ let mk_total_interpretation_6
     (e5:embedding 't5)
     (e6:embedding 't6)
     (er:embedding 'r)
-    (psc:Cfg.psc)
+    (psc:PO.psc)
     (ncb:norm_cb)
     (args:args)
   : option term
@@ -1794,7 +1795,7 @@ let mk_total_interpretation_6
     BU.bind_opt (unembed e5 a5 ncb) (fun a5 ->
     BU.bind_opt (unembed e6 a6 ncb) (fun a6 ->
     let r = interp_ctx name (fun () -> f a1 a2 a3 a4 a5 a6) in
-    Some (embed er (Cfg.psc_range psc) r ncb)))))))
+    Some (embed er (PO.psc_range psc) r ncb)))))))
   | _ ->
     None
 
@@ -1809,7 +1810,7 @@ let mk_total_interpretation_7
     (e6:embedding 't6)
     (e7:embedding 't7)
     (er:embedding 'r)
-    (psc:Cfg.psc)
+    (psc:PO.psc)
     (ncb:norm_cb)
     (args:args)
   : option term
@@ -1824,7 +1825,7 @@ let mk_total_interpretation_7
     BU.bind_opt (unembed e6 a6 ncb) (fun a6 ->
     BU.bind_opt (unembed e7 a7 ncb) (fun a7 ->
     let r = interp_ctx name (fun () -> f a1 a2 a3 a4 a5 a6 a7) in
-    Some (embed er (Cfg.psc_range psc) r ncb))))))))
+    Some (embed er (PO.psc_range psc) r ncb))))))))
   | _ ->
     None
 
@@ -1840,7 +1841,7 @@ let mk_total_interpretation_8
     (e7:embedding 't7)
     (e8:embedding 't8)
     (er:embedding 'r)
-    (psc:Cfg.psc)
+    (psc:PO.psc)
     (ncb:norm_cb)
     (args:args)
   : option term
@@ -1856,7 +1857,7 @@ let mk_total_interpretation_8
     BU.bind_opt (unembed e7 a7 ncb) (fun a7 ->
     BU.bind_opt (unembed e8 a8 ncb) (fun a8 ->
     let r = interp_ctx name (fun () -> f a1 a2 a3 a4 a5 a6 a7 a8) in
-    Some (embed er (Cfg.psc_range psc) r ncb)))))))))
+    Some (embed er (PO.psc_range psc) r ncb)))))))))
   | _ ->
     None
 
@@ -1873,7 +1874,7 @@ let mk_total_interpretation_9
     (e8:embedding 't8)
     (e9:embedding 't9)
     (er:embedding 'r)
-    (psc:Cfg.psc)
+    (psc:PO.psc)
     (ncb:norm_cb)
     (args:args)
   : option term
@@ -1890,7 +1891,7 @@ let mk_total_interpretation_9
     BU.bind_opt (unembed e8 a8 ncb) (fun a8 ->
     BU.bind_opt (unembed e9 a9 ncb) (fun a9 ->
     let r = interp_ctx name (fun () -> f a1 a2 a3 a4 a5 a6 a7 a8 a9) in
-    Some (embed er (Cfg.psc_range psc) r ncb))))))))))
+    Some (embed er (PO.psc_range psc) r ncb))))))))))
   | _ ->
     None
 
@@ -1908,7 +1909,7 @@ let mk_total_interpretation_10
     (e9:embedding 't9)
     (e10:embedding 't10)
     (er:embedding 'r)
-    (psc:Cfg.psc)
+    (psc:PO.psc)
     (ncb:norm_cb)
     (args:args)
   : option term
@@ -1926,7 +1927,7 @@ let mk_total_interpretation_10
     BU.bind_opt (unembed e9 a9 ncb) (fun a9 ->
     BU.bind_opt (unembed e10 a10 ncb) (fun a10 ->
     let r = interp_ctx name (fun () -> f a1 a2 a3 a4 a5 a6 a7 a8 a9 a10) in
-    Some (embed er (Cfg.psc_range psc) r ncb)))))))))))
+    Some (embed er (PO.psc_range psc) r ncb)))))))))))
   | _ ->
     None
 
@@ -1945,7 +1946,7 @@ let mk_total_interpretation_11
     (e10:embedding 't10)
     (e11:embedding 't11)
     (er:embedding 'r)
-    (psc:Cfg.psc)
+    (psc:PO.psc)
     (ncb:norm_cb)
     (args:args)
   : option term
@@ -1964,7 +1965,7 @@ let mk_total_interpretation_11
     BU.bind_opt (unembed e10 a10 ncb) (fun a10 ->
     BU.bind_opt (unembed e11 a11 ncb) (fun a11 ->
     let r = interp_ctx name (fun () -> f a1 a2 a3 a4 a5 a6 a7 a8 a9 a10 a11) in
-    Some (embed er (Cfg.psc_range psc) r ncb))))))))))))
+    Some (embed er (PO.psc_range psc) r ncb))))))))))))
   | _ ->
     None
 
@@ -1984,7 +1985,7 @@ let mk_total_interpretation_12
     (e11:embedding 't11)
     (e12:embedding 't12)
     (er:embedding 'r)
-    (psc:Cfg.psc)
+    (psc:PO.psc)
     (ncb:norm_cb)
     (args:args)
   : option term
@@ -2004,7 +2005,7 @@ let mk_total_interpretation_12
     BU.bind_opt (unembed e11 a11 ncb) (fun a11 ->
     BU.bind_opt (unembed e12 a12 ncb) (fun a12 ->
     let r = interp_ctx name (fun () -> f a1 a2 a3 a4 a5 a6 a7 a8 a9 a10 a11 a12) in
-    Some (embed er (Cfg.psc_range psc) r ncb)))))))))))))
+    Some (embed er (PO.psc_range psc) r ncb)))))))))))))
   | _ ->
     None
 
@@ -2025,7 +2026,7 @@ let mk_total_interpretation_13
     (e12:embedding 't12)
     (e13:embedding 't13)
     (er:embedding 'r)
-    (psc:Cfg.psc)
+    (psc:PO.psc)
     (ncb:norm_cb)
     (args:args)
   : option term
@@ -2046,7 +2047,7 @@ let mk_total_interpretation_13
     BU.bind_opt (unembed e12 a12 ncb) (fun a12 ->
     BU.bind_opt (unembed e13 a13 ncb) (fun a13 ->
     let r = interp_ctx name (fun () -> f a1 a2 a3 a4 a5 a6 a7 a8 a9 a10 a11 a12 a13) in
-    Some (embed er (Cfg.psc_range psc) r ncb))))))))))))))
+    Some (embed er (PO.psc_range psc) r ncb))))))))))))))
   | _ ->
     None
 
@@ -2068,7 +2069,7 @@ let mk_total_interpretation_14
     (e13:embedding 't13)
     (e14:embedding 't14)
     (er:embedding 'r)
-    (psc:Cfg.psc)
+    (psc:PO.psc)
     (ncb:norm_cb)
     (args:args)
   : option term
@@ -2090,7 +2091,7 @@ let mk_total_interpretation_14
     BU.bind_opt (unembed e13 a13 ncb) (fun a13 ->
     BU.bind_opt (unembed e14 a14 ncb) (fun a14 ->
     let r = interp_ctx name (fun () -> f a1 a2 a3 a4 a5 a6 a7 a8 a9 a10 a11 a12 a13 a14) in
-    Some (embed er (Cfg.psc_range psc) r ncb)))))))))))))))
+    Some (embed er (PO.psc_range psc) r ncb)))))))))))))))
   | _ ->
     None
 
@@ -2113,7 +2114,7 @@ let mk_total_interpretation_15
     (e14:embedding 't14)
     (e15:embedding 't15)
     (er:embedding 'r)
-    (psc:Cfg.psc)
+    (psc:PO.psc)
     (ncb:norm_cb)
     (args:args)
   : option term
@@ -2136,7 +2137,7 @@ let mk_total_interpretation_15
     BU.bind_opt (unembed e14 a14 ncb) (fun a14 ->
     BU.bind_opt (unembed e15 a15 ncb) (fun a15 ->
     let r = interp_ctx name (fun () -> f a1 a2 a3 a4 a5 a6 a7 a8 a9 a10 a11 a12 a13 a14 a15) in
-    Some (embed er (Cfg.psc_range psc) r ncb))))))))))))))))
+    Some (embed er (PO.psc_range psc) r ncb))))))))))))))))
   | _ ->
     None
 
@@ -2160,7 +2161,7 @@ let mk_total_interpretation_16
     (e15:embedding 't15)
     (e16:embedding 't16)
     (er:embedding 'r)
-    (psc:Cfg.psc)
+    (psc:PO.psc)
     (ncb:norm_cb)
     (args:args)
   : option term
@@ -2184,7 +2185,7 @@ let mk_total_interpretation_16
     BU.bind_opt (unembed e15 a15 ncb) (fun a15 ->
     BU.bind_opt (unembed e16 a16 ncb) (fun a16 ->
     let r = interp_ctx name (fun () -> f a1 a2 a3 a4 a5 a6 a7 a8 a9 a10 a11 a12 a13 a14 a15 a16) in
-    Some (embed er (Cfg.psc_range psc) r ncb)))))))))))))))))
+    Some (embed er (PO.psc_range psc) r ncb)))))))))))))))))
   | _ ->
     None
 
@@ -2209,7 +2210,7 @@ let mk_total_interpretation_17
     (e16:embedding 't16)
     (e17:embedding 't17)
     (er:embedding 'r)
-    (psc:Cfg.psc)
+    (psc:PO.psc)
     (ncb:norm_cb)
     (args:args)
   : option term
@@ -2234,7 +2235,7 @@ let mk_total_interpretation_17
     BU.bind_opt (unembed e16 a16 ncb) (fun a16 ->
     BU.bind_opt (unembed e17 a17 ncb) (fun a17 ->
     let r = interp_ctx name (fun () -> f a1 a2 a3 a4 a5 a6 a7 a8 a9 a10 a11 a12 a13 a14 a15 a16 a17) in
-    Some (embed er (Cfg.psc_range psc) r ncb))))))))))))))))))
+    Some (embed er (PO.psc_range psc) r ncb))))))))))))))))))
   | _ ->
     None
 
@@ -2260,7 +2261,7 @@ let mk_total_interpretation_18
     (e17:embedding 't17)
     (e18:embedding 't18)
     (er:embedding 'r)
-    (psc:Cfg.psc)
+    (psc:PO.psc)
     (ncb:norm_cb)
     (args:args)
   : option term
@@ -2286,7 +2287,7 @@ let mk_total_interpretation_18
     BU.bind_opt (unembed e17 a17 ncb) (fun a17 ->
     BU.bind_opt (unembed e18 a18 ncb) (fun a18 ->
     let r = interp_ctx name (fun () -> f a1 a2 a3 a4 a5 a6 a7 a8 a9 a10 a11 a12 a13 a14 a15 a16 a17 a18) in
-    Some (embed er (Cfg.psc_range psc) r ncb)))))))))))))))))))
+    Some (embed er (PO.psc_range psc) r ncb)))))))))))))))))))
   | _ ->
     None
 
@@ -2313,7 +2314,7 @@ let mk_total_interpretation_19
     (e18:embedding 't18)
     (e19:embedding 't19)
     (er:embedding 'r)
-    (psc:Cfg.psc)
+    (psc:PO.psc)
     (ncb:norm_cb)
     (args:args)
   : option term
@@ -2340,7 +2341,7 @@ let mk_total_interpretation_19
     BU.bind_opt (unembed e18 a18 ncb) (fun a18 ->
     BU.bind_opt (unembed e19 a19 ncb) (fun a19 ->
     let r = interp_ctx name (fun () -> f a1 a2 a3 a4 a5 a6 a7 a8 a9 a10 a11 a12 a13 a14 a15 a16 a17 a18 a19) in
-    Some (embed er (Cfg.psc_range psc) r ncb))))))))))))))))))))
+    Some (embed er (PO.psc_range psc) r ncb))))))))))))))))))))
   | _ ->
     None
 
@@ -2368,7 +2369,7 @@ let mk_total_interpretation_20
     (e19:embedding 't19)
     (e20:embedding 't20)
     (er:embedding 'r)
-    (psc:Cfg.psc)
+    (psc:PO.psc)
     (ncb:norm_cb)
     (args:args)
   : option term
@@ -2396,7 +2397,7 @@ let mk_total_interpretation_20
     BU.bind_opt (unembed e19 a19 ncb) (fun a19 ->
     BU.bind_opt (unembed e20 a20 ncb) (fun a20 ->
     let r = interp_ctx name (fun () -> f a1 a2 a3 a4 a5 a6 a7 a8 a9 a10 a11 a12 a13 a14 a15 a16 a17 a18 a19 a20) in
-    Some (embed er (Cfg.psc_range psc) r ncb)))))))))))))))))))))
+    Some (embed er (PO.psc_range psc) r ncb)))))))))))))))))))))
   | _ ->
     None
 
@@ -3129,7 +3130,7 @@ let mk_tac_step_1
   (nt : 'nt1 -> tac 'nr)
   (ne1:NBET.embedding 'nt1)
   (ner:NBET.embedding 'nr)
-  : Cfg.primitive_step
+  : PO.primitive_step
   =
     mk name 2 nunivs
       (mk_tactic_interpretation_1 name t e1 er)
@@ -3146,7 +3147,7 @@ let mk_tac_step_2
   (ne1:NBET.embedding 'nt1)
   (ne2:NBET.embedding 'nt2)
   (ner:NBET.embedding 'nr)
-  : Cfg.primitive_step
+  : PO.primitive_step
   =
     mk name 3 nunivs
       (mk_tactic_interpretation_2 name t e1 e2 er)
@@ -3165,7 +3166,7 @@ let mk_tac_step_3
   (ne2:NBET.embedding 'nt2)
   (ne3:NBET.embedding 'nt3)
   (ner:NBET.embedding 'nr)
-  : Cfg.primitive_step
+  : PO.primitive_step
   =
     mk name 4 nunivs
       (mk_tactic_interpretation_3 name t e1 e2 e3 er)
@@ -3186,7 +3187,7 @@ let mk_tac_step_4
   (ne3:NBET.embedding 'nt3)
   (ne4:NBET.embedding 'nt4)
   (ner:NBET.embedding 'nr)
-  : Cfg.primitive_step
+  : PO.primitive_step
   =
     mk name 5 nunivs
       (mk_tactic_interpretation_4 name t e1 e2 e3 e4 er)
@@ -3209,7 +3210,7 @@ let mk_tac_step_5
   (ne4:NBET.embedding 'nt4)
   (ne5:NBET.embedding 'nt5)
   (ner:NBET.embedding 'nr)
-  : Cfg.primitive_step
+  : PO.primitive_step
   =
     mk name 6 nunivs
       (mk_tactic_interpretation_5 name t e1 e2 e3 e4 e5 er)
@@ -3234,7 +3235,7 @@ let mk_tac_step_6
   (ne5:NBET.embedding 'nt5)
   (ne6:NBET.embedding 'nt6)
   (ner:NBET.embedding 'nr)
-  : Cfg.primitive_step
+  : PO.primitive_step
   =
     mk name 7 nunivs
       (mk_tactic_interpretation_6 name t e1 e2 e3 e4 e5 e6 er)
@@ -3261,7 +3262,7 @@ let mk_tac_step_7
   (ne6:NBET.embedding 'nt6)
   (ne7:NBET.embedding 'nt7)
   (ner:NBET.embedding 'nr)
-  : Cfg.primitive_step
+  : PO.primitive_step
   =
     mk name 8 nunivs
       (mk_tactic_interpretation_7 name t e1 e2 e3 e4 e5 e6 e7 er)
@@ -3290,7 +3291,7 @@ let mk_tac_step_8
   (ne7:NBET.embedding 'nt7)
   (ne8:NBET.embedding 'nt8)
   (ner:NBET.embedding 'nr)
-  : Cfg.primitive_step
+  : PO.primitive_step
   =
     mk name 9 nunivs
       (mk_tactic_interpretation_8 name t e1 e2 e3 e4 e5 e6 e7 e8 er)
@@ -3321,7 +3322,7 @@ let mk_tac_step_9
   (ne8:NBET.embedding 'nt8)
   (ne9:NBET.embedding 'nt9)
   (ner:NBET.embedding 'nr)
-  : Cfg.primitive_step
+  : PO.primitive_step
   =
     mk name 10 nunivs
       (mk_tactic_interpretation_9 name t e1 e2 e3 e4 e5 e6 e7 e8 e9 er)
@@ -3354,7 +3355,7 @@ let mk_tac_step_10
   (ne9:NBET.embedding 'nt9)
   (ne10:NBET.embedding 'nt10)
   (ner:NBET.embedding 'nr)
-  : Cfg.primitive_step
+  : PO.primitive_step
   =
     mk name 11 nunivs
       (mk_tactic_interpretation_10 name t e1 e2 e3 e4 e5 e6 e7 e8 e9 e10 er)
@@ -3389,7 +3390,7 @@ let mk_tac_step_11
   (ne10:NBET.embedding 'nt10)
   (ne11:NBET.embedding 'nt11)
   (ner:NBET.embedding 'nr)
-  : Cfg.primitive_step
+  : PO.primitive_step
   =
     mk name 12 nunivs
       (mk_tactic_interpretation_11 name t e1 e2 e3 e4 e5 e6 e7 e8 e9 e10 e11 er)
@@ -3426,7 +3427,7 @@ let mk_tac_step_12
   (ne11:NBET.embedding 'nt11)
   (ne12:NBET.embedding 'nt12)
   (ner:NBET.embedding 'nr)
-  : Cfg.primitive_step
+  : PO.primitive_step
   =
     mk name 13 nunivs
       (mk_tactic_interpretation_12 name t e1 e2 e3 e4 e5 e6 e7 e8 e9 e10 e11 e12 er)
@@ -3465,7 +3466,7 @@ let mk_tac_step_13
   (ne12:NBET.embedding 'nt12)
   (ne13:NBET.embedding 'nt13)
   (ner:NBET.embedding 'nr)
-  : Cfg.primitive_step
+  : PO.primitive_step
   =
     mk name 14 nunivs
       (mk_tactic_interpretation_13 name t e1 e2 e3 e4 e5 e6 e7 e8 e9 e10 e11 e12 e13 er)
@@ -3506,7 +3507,7 @@ let mk_tac_step_14
   (ne13:NBET.embedding 'nt13)
   (ne14:NBET.embedding 'nt14)
   (ner:NBET.embedding 'nr)
-  : Cfg.primitive_step
+  : PO.primitive_step
   =
     mk name 15 nunivs
       (mk_tactic_interpretation_14 name t e1 e2 e3 e4 e5 e6 e7 e8 e9 e10 e11 e12 e13 e14 er)
@@ -3549,7 +3550,7 @@ let mk_tac_step_15
   (ne14:NBET.embedding 'nt14)
   (ne15:NBET.embedding 'nt15)
   (ner:NBET.embedding 'nr)
-  : Cfg.primitive_step
+  : PO.primitive_step
   =
     mk name 16 nunivs
       (mk_tactic_interpretation_15 name t e1 e2 e3 e4 e5 e6 e7 e8 e9 e10 e11 e12 e13 e14 e15 er)
@@ -3594,7 +3595,7 @@ let mk_tac_step_16
   (ne15:NBET.embedding 'nt15)
   (ne16:NBET.embedding 'nt16)
   (ner:NBET.embedding 'nr)
-  : Cfg.primitive_step
+  : PO.primitive_step
   =
     mk name 17 nunivs
       (mk_tactic_interpretation_16 name t e1 e2 e3 e4 e5 e6 e7 e8 e9 e10 e11 e12 e13 e14 e15 e16 er)
@@ -3641,7 +3642,7 @@ let mk_tac_step_17
   (ne16:NBET.embedding 'nt16)
   (ne17:NBET.embedding 'nt17)
   (ner:NBET.embedding 'nr)
-  : Cfg.primitive_step
+  : PO.primitive_step
   =
     mk name 18 nunivs
       (mk_tactic_interpretation_17 name t e1 e2 e3 e4 e5 e6 e7 e8 e9 e10 e11 e12 e13 e14 e15 e16 e17 er)
@@ -3690,7 +3691,7 @@ let mk_tac_step_18
   (ne17:NBET.embedding 'nt17)
   (ne18:NBET.embedding 'nt18)
   (ner:NBET.embedding 'nr)
-  : Cfg.primitive_step
+  : PO.primitive_step
   =
     mk name 19 nunivs
       (mk_tactic_interpretation_18 name t e1 e2 e3 e4 e5 e6 e7 e8 e9 e10 e11 e12 e13 e14 e15 e16 e17 e18 er)
@@ -3741,7 +3742,7 @@ let mk_tac_step_19
   (ne18:NBET.embedding 'nt18)
   (ne19:NBET.embedding 'nt19)
   (ner:NBET.embedding 'nr)
-  : Cfg.primitive_step
+  : PO.primitive_step
   =
     mk name 20 nunivs
       (mk_tactic_interpretation_19 name t e1 e2 e3 e4 e5 e6 e7 e8 e9 e10 e11 e12 e13 e14 e15 e16 e17 e18 e19 er)
@@ -3794,7 +3795,7 @@ let mk_tac_step_20
   (ne19:NBET.embedding 'nt19)
   (ne20:NBET.embedding 'nt20)
   (ner:NBET.embedding 'nr)
-  : Cfg.primitive_step
+  : PO.primitive_step
   =
     mk name 21 nunivs
       (mk_tactic_interpretation_20 name t e1 e2 e3 e4 e5 e6 e7 e8 e9 e10 e11 e12 e13 e14 e15 e16 e17 e18 e19 e20 er)
@@ -3809,7 +3810,7 @@ let mk_total_step_1
   (nf : 'nt1 -> 'nr)
   (ne1:NBET.embedding 'nt1)
   (ner:NBET.embedding 'nr)
-  : Cfg.primitive_step
+  : PO.primitive_step
   =
     mk name 1 nunivs
       (mk_total_interpretation_1 name f e1 er)
@@ -3826,7 +3827,7 @@ let mk_total_step_2
   (ne1:NBET.embedding 'nt1)
   (ne2:NBET.embedding 'nt2)
   (ner:NBET.embedding 'nr)
-  : Cfg.primitive_step
+  : PO.primitive_step
   =
     mk name 2 nunivs
       (mk_total_interpretation_2 name f e1 e2 er)
@@ -3845,7 +3846,7 @@ let mk_total_step_3
   (ne2:NBET.embedding 'nt2)
   (ne3:NBET.embedding 'nt3)
   (ner:NBET.embedding 'nr)
-  : Cfg.primitive_step
+  : PO.primitive_step
   =
     mk name 3 nunivs
       (mk_total_interpretation_3 name f e1 e2 e3 er)
@@ -3866,7 +3867,7 @@ let mk_total_step_4
   (ne3:NBET.embedding 'nt3)
   (ne4:NBET.embedding 'nt4)
   (ner:NBET.embedding 'nr)
-  : Cfg.primitive_step
+  : PO.primitive_step
   =
     mk name 4 nunivs
       (mk_total_interpretation_4 name f e1 e2 e3 e4 er)
@@ -3889,7 +3890,7 @@ let mk_total_step_5
   (ne4:NBET.embedding 'nt4)
   (ne5:NBET.embedding 'nt5)
   (ner:NBET.embedding 'nr)
-  : Cfg.primitive_step
+  : PO.primitive_step
   =
     mk name 5 nunivs
       (mk_total_interpretation_5 name f e1 e2 e3 e4 e5 er)
@@ -3914,7 +3915,7 @@ let mk_total_step_6
   (ne5:NBET.embedding 'nt5)
   (ne6:NBET.embedding 'nt6)
   (ner:NBET.embedding 'nr)
-  : Cfg.primitive_step
+  : PO.primitive_step
   =
     mk name 6 nunivs
       (mk_total_interpretation_6 name f e1 e2 e3 e4 e5 e6 er)
@@ -3941,7 +3942,7 @@ let mk_total_step_7
   (ne6:NBET.embedding 'nt6)
   (ne7:NBET.embedding 'nt7)
   (ner:NBET.embedding 'nr)
-  : Cfg.primitive_step
+  : PO.primitive_step
   =
     mk name 7 nunivs
       (mk_total_interpretation_7 name f e1 e2 e3 e4 e5 e6 e7 er)
@@ -3970,7 +3971,7 @@ let mk_total_step_8
   (ne7:NBET.embedding 'nt7)
   (ne8:NBET.embedding 'nt8)
   (ner:NBET.embedding 'nr)
-  : Cfg.primitive_step
+  : PO.primitive_step
   =
     mk name 8 nunivs
       (mk_total_interpretation_8 name f e1 e2 e3 e4 e5 e6 e7 e8 er)
@@ -4001,7 +4002,7 @@ let mk_total_step_9
   (ne8:NBET.embedding 'nt8)
   (ne9:NBET.embedding 'nt9)
   (ner:NBET.embedding 'nr)
-  : Cfg.primitive_step
+  : PO.primitive_step
   =
     mk name 9 nunivs
       (mk_total_interpretation_9 name f e1 e2 e3 e4 e5 e6 e7 e8 e9 er)
@@ -4034,7 +4035,7 @@ let mk_total_step_10
   (ne9:NBET.embedding 'nt9)
   (ne10:NBET.embedding 'nt10)
   (ner:NBET.embedding 'nr)
-  : Cfg.primitive_step
+  : PO.primitive_step
   =
     mk name 10 nunivs
       (mk_total_interpretation_10 name f e1 e2 e3 e4 e5 e6 e7 e8 e9 e10 er)
@@ -4069,7 +4070,7 @@ let mk_total_step_11
   (ne10:NBET.embedding 'nt10)
   (ne11:NBET.embedding 'nt11)
   (ner:NBET.embedding 'nr)
-  : Cfg.primitive_step
+  : PO.primitive_step
   =
     mk name 11 nunivs
       (mk_total_interpretation_11 name f e1 e2 e3 e4 e5 e6 e7 e8 e9 e10 e11 er)
@@ -4106,7 +4107,7 @@ let mk_total_step_12
   (ne11:NBET.embedding 'nt11)
   (ne12:NBET.embedding 'nt12)
   (ner:NBET.embedding 'nr)
-  : Cfg.primitive_step
+  : PO.primitive_step
   =
     mk name 12 nunivs
       (mk_total_interpretation_12 name f e1 e2 e3 e4 e5 e6 e7 e8 e9 e10 e11 e12 er)
@@ -4145,7 +4146,7 @@ let mk_total_step_13
   (ne12:NBET.embedding 'nt12)
   (ne13:NBET.embedding 'nt13)
   (ner:NBET.embedding 'nr)
-  : Cfg.primitive_step
+  : PO.primitive_step
   =
     mk name 13 nunivs
       (mk_total_interpretation_13 name f e1 e2 e3 e4 e5 e6 e7 e8 e9 e10 e11 e12 e13 er)
@@ -4186,7 +4187,7 @@ let mk_total_step_14
   (ne13:NBET.embedding 'nt13)
   (ne14:NBET.embedding 'nt14)
   (ner:NBET.embedding 'nr)
-  : Cfg.primitive_step
+  : PO.primitive_step
   =
     mk name 14 nunivs
       (mk_total_interpretation_14 name f e1 e2 e3 e4 e5 e6 e7 e8 e9 e10 e11 e12 e13 e14 er)
@@ -4229,7 +4230,7 @@ let mk_total_step_15
   (ne14:NBET.embedding 'nt14)
   (ne15:NBET.embedding 'nt15)
   (ner:NBET.embedding 'nr)
-  : Cfg.primitive_step
+  : PO.primitive_step
   =
     mk name 15 nunivs
       (mk_total_interpretation_15 name f e1 e2 e3 e4 e5 e6 e7 e8 e9 e10 e11 e12 e13 e14 e15 er)
@@ -4274,7 +4275,7 @@ let mk_total_step_16
   (ne15:NBET.embedding 'nt15)
   (ne16:NBET.embedding 'nt16)
   (ner:NBET.embedding 'nr)
-  : Cfg.primitive_step
+  : PO.primitive_step
   =
     mk name 16 nunivs
       (mk_total_interpretation_16 name f e1 e2 e3 e4 e5 e6 e7 e8 e9 e10 e11 e12 e13 e14 e15 e16 er)
@@ -4321,7 +4322,7 @@ let mk_total_step_17
   (ne16:NBET.embedding 'nt16)
   (ne17:NBET.embedding 'nt17)
   (ner:NBET.embedding 'nr)
-  : Cfg.primitive_step
+  : PO.primitive_step
   =
     mk name 17 nunivs
       (mk_total_interpretation_17 name f e1 e2 e3 e4 e5 e6 e7 e8 e9 e10 e11 e12 e13 e14 e15 e16 e17 er)
@@ -4370,7 +4371,7 @@ let mk_total_step_18
   (ne17:NBET.embedding 'nt17)
   (ne18:NBET.embedding 'nt18)
   (ner:NBET.embedding 'nr)
-  : Cfg.primitive_step
+  : PO.primitive_step
   =
     mk name 18 nunivs
       (mk_total_interpretation_18 name f e1 e2 e3 e4 e5 e6 e7 e8 e9 e10 e11 e12 e13 e14 e15 e16 e17 e18 er)
@@ -4421,7 +4422,7 @@ let mk_total_step_19
   (ne18:NBET.embedding 'nt18)
   (ne19:NBET.embedding 'nt19)
   (ner:NBET.embedding 'nr)
-  : Cfg.primitive_step
+  : PO.primitive_step
   =
     mk name 19 nunivs
       (mk_total_interpretation_19 name f e1 e2 e3 e4 e5 e6 e7 e8 e9 e10 e11 e12 e13 e14 e15 e16 e17 e18 e19 er)
@@ -4474,7 +4475,7 @@ let mk_total_step_20
   (ne19:NBET.embedding 'nt19)
   (ne20:NBET.embedding 'nt20)
   (ner:NBET.embedding 'nr)
-  : Cfg.primitive_step
+  : PO.primitive_step
   =
     mk name 20 nunivs
       (mk_total_interpretation_20 name f e1 e2 e3 e4 e5 e6 e7 e8 e9 e10 e11 e12 e13 e14 e15 e16 e17 e18 e19 e20 er)
