src/typechecker/FStar.TypeChecker.Primops.fsti
@@ -1,0 +1,43 @@
+module FStar.TypeChecker.Primops
+
+(* This module just contains the list of all builtin primitive steps
+with their implementations. *)
+
+open FStar
+open FStar.Compiler
+open FStar.Compiler.Effect
+open FStar.Compiler.List
+open FStar.Syntax.Syntax
+
+module EMB = FStar.Syntax.Embeddings
+module NBE = FStar.TypeChecker.NBETerm
+
+type psc = {
+     psc_range : FStar.Compiler.Range.range;
+     psc_subst : unit -> subst_t // potentially expensive, so thunked
+}
+
+val null_psc : psc
+val psc_range : psc -> FStar.Compiler.Range.range
+val psc_subst : psc -> subst_t
+
+type primitive_step = {
+    name:FStar.Ident.lid;
+    arity:int;
+    univ_arity:int; // universe arity
+    auto_reflect:option int;
+    strong_reduction_ok:bool;
+    requires_binder_substitution:bool;
+    renorm_after:bool; // whether the result of this primop must possibly undergo more normalization
+    interpretation:(psc -> FStar.Syntax.Embeddings.norm_cb -> universes -> args -> option term);
+    interpretation_nbe:(NBE.nbe_cbs -> universes -> NBE.args -> option NBE.t)
+}
+
+(* Some helpers for the NBE. Does not really belong in this module. *)
+val embed_simple: EMB.embedding 'a -> Range.range -> 'a -> term
+val try_unembed_simple: EMB.embedding 'a -> term -> option 'a
+
+val built_in_primitive_steps_list
+  : list primitive_step
+val equality_ops_list
+  : list primitive_step
